[michocoq] Enforce concrete maps and big maps to be sorted by construction
Solves #28.

src/michocoq/map.v
@@ -24,6 +24,7 @@
 
 Require set.
 Require Import error.
+Require Eqdep_dec.
 Import error.Notations.
 
 Section map.
@@ -55,553 +56,912 @@ Section map.
       + right. reflexivity.
   Qed.
 
+  Lemma gt_irrefl a : compare a a <> Gt.
+  Proof.
+    rewrite compare_refl.
+    congruence.
+  Qed.
+
+  Lemma lt_irrefl a : compare a a <> Lt.
+  Proof.
+    rewrite compare_refl.
+    congruence.
+  Qed.
+
+  Lemma lt_antisym a b : compare a b = Lt -> compare b a <> Lt.
+  Proof.
+    intros H1 H2.
+    apply (lt_irrefl a).
+    apply (lt_trans a b a); assumption.
+  Qed.
+
+  Lemma gt_rev a b : compare a b = Gt -> compare b a = Lt.
+  Proof.
+    case_eq (compare b a).
+    - intro He.
+      apply compare_eq_iff in He.
+      subst b.
+      rewrite compare_refl.
+      congruence.
+    - intuition.
+    - intros H1 H2.
+      exfalso.
+      apply (gt_irrefl a).
+      apply (gt_trans a b a); assumption.
+  Qed.
+
+  Lemma lt_rev a b : compare a b = Lt -> compare b a = Gt.
+  Proof.
+    case_eq (compare b a).
+    - intro He.
+      apply compare_eq_iff in He.
+      subst b.
+      rewrite compare_refl.
+      congruence.
+    - intros H1 H2.
+      exfalso.
+      apply (lt_irrefl a).
+      apply (lt_trans a b a); assumption.
+    - intuition.
+  Qed.
+
+  Lemma trans_lt_le k1 k2 k3 : compare k1 k2 = Lt -> compare k3 k2 <> Lt -> compare k1 k3 = Lt.
+  Proof.
+    case_eq (compare k3 k2).
+    - intros H23 H12 _.
+      apply compare_eq_iff in H23.
+      congruence.
+    - congruence.
+    - intros H23 H12 _.
+      apply gt_rev in H23.
+      apply (lt_trans k1 k2 k3); assumption.
+  Qed.
+
+  Lemma eq_not_lt a b : compare a b = Eq -> compare a b <> Lt.
+  Proof.
+    congruence.
+  Qed.
+
+  Lemma gt_not_lt a b : compare a b = Gt -> compare a b <> Lt.
+  Proof.
+    congruence.
+  Qed.
+
+  Lemma eq_dec (a b : A) : {a = b} + {a <> b}.
+  Proof.
+    case_eq (compare a b).
+    - intro H.
+      left.
+      apply compare_eq_iff.
+      assumption.
+    - intro Hlt. right. intro He.
+      apply compare_eq_iff in He.
+      congruence.
+    - intro Hgt. right. intro He.
+      apply compare_eq_iff in He.
+      congruence.
+  Defined.
+
   Definition map_compare (x_ y_ : A * B) :=
     match x_, y_ with (x, _), (y, _) => compare x y end.
 
-  Definition map := set.set (A * B) map_compare.
+  (* a [sorted_map_above k] represents a non-empty map whose smallest key is [k] *)
+  Inductive sorted_map_above : A -> Set :=
+  | sorted_map_sing k : sorted_map_above k
+  | sorted_map_cons k1 k2 (v2 : B)
+                    (H : compare k1 k2 = Lt) :
+      sorted_map_above k2 -> sorted_map_above k1.
+  Inductive sorted_map : Set :=
+  | sorted_map_nil : sorted_map
+  | sorted_map_nonnil k (v : B) : sorted_map_above k -> sorted_map.
 
-  Fixpoint list_mem (x : A) (l : list (A * B)) : bool :=
-    match l with
-    | nil => false
-    | cons y l =>
-      let (k, v) := y in
-      match compare x k with
-      | Lt => false
-      | Eq => true
-      | Gt => list_mem x l
+  Definition map := sorted_map.
+
+  Fixpoint mem_above (k : A) (x : A) (m : sorted_map_above k) : bool :=
+    match compare x k with
+    | Lt => false
+    | Eq => true
+    | Gt =>
+      match m with
+      | sorted_map_sing _ => false
+      | sorted_map_cons _ k _ _ m =>
+        mem_above k x m
       end
     end.
 
   Definition mem (x : A) (m : map) : bool :=
-    let (l, _) := m in list_mem x l.
-
-  Fixpoint list_remove (x : A) (l : list (A * B)) : list (A * B) :=
-    match l with
-    | nil => nil
-    | cons y l =>
-      let (k, v) := y in
-      match compare x k with
-      | Lt => cons y l
-      | Eq => l
-      | Gt => cons y (list_remove x l)
-      end
+    match m with
+    | sorted_map_nil => false
+    | sorted_map_nonnil k _ m =>
+      mem_above k x m
     end.
 
-  Lemma remove_in x v y l : List.In (x, v) (list_remove y l) -> List.In (x, v) l.
-  Proof.
-    induction l as [|(z, v') l]; simpl.
-    - auto.
-    - case_eq (compare y z).
-      + intuition.
-      + intros Hlt Hin.
-        simpl in Hin.
-        assumption.
-      + intros Hgt Hin.
-        simpl in Hin.
-        intuition.
-  Qed.
-
-  Fixpoint list_replace (x : A) (v : B) (l : list (A * B)) : list (A * B) :=
-    match l with
-    | nil => cons (x, v) nil
-    | cons y l =>
-      let (k, _) := y in
-      match compare x k with
-      | Lt => cons (x, v) (cons y l)
-      | Eq => cons (x, v) l
-      | Gt => cons y (list_replace x v l)
-      end
-    end.
-
-  Lemma list_replace_same x v v' l :
-    Sorted.StronglySorted (set.lt _ map_compare) l ->
-    List.In (x, v) (list_replace x v' l) <-> v = v'.
-  Proof.
-    induction l as [|(y, v'') l].
-    - simpl.
-      intuition congruence.
-    - simpl.
-      case_eq (compare x y).
-      + intros He Hs.
-        apply Sorted.StronglySorted_inv in Hs.
-        destruct Hs as (Hs, Hf).
-        rewrite compare_eq_iff in He.
-        simpl.
-        split.
-        * intros [He2|Hin].
-          {
-            congruence.
-          }
-          {
-            rewrite List.Forall_forall in Hf.
-            specialize (Hf (x, v) Hin).
-            unfold set.lt, map_compare in Hf.
-            symmetry in He.
-            rewrite <- compare_eq_iff in He.
-            congruence.
-          }
-        * intro; left; congruence.
-      + intros Hlt Hs.
-        apply Sorted.StronglySorted_inv in Hs.
-        destruct Hs as (Hs, Hf).
-        simpl.
-        split.
-        * intros [He2|Hin].
-          {
-            congruence.
-          }
-          {
-            rewrite List.Forall_forall in Hf.
-            specialize (Hf (x, v)).
-            unfold set.lt, map_compare in Hf.
-            simpl in Hin.
-            destruct Hin as [He|Hin].
-            - injection He.
-              intros _ He2.
-              symmetry in He2.
-              rewrite <- compare_eq_iff in He2.
-              congruence.
-            - specialize (Hf Hin).
-              assert (compare x x = Lt) by (apply (lt_trans x y x); assumption).
-              assert (compare x x = Eq) by (apply (compare_eq_iff x x); reflexivity).
-              congruence.
-          }
-        * intro He.
-          destruct He.
-          left; reflexivity.
-      + simpl.
-        intros Hgt Hs.
-        rewrite IHl.
-        * split; [|intuition].
-          intros [He|He]; [|auto].
-          injection He.
-          intros _ He2.
-          symmetry in He2.
-          rewrite <- compare_eq_iff in He2.
-          congruence.
-        * inversion Hs.
-          assumption.
-  Qed.
-
-  Lemma list_replace_diff x v y v' l :
-    Sorted.StronglySorted (set.lt _ map_compare) l ->
-    x <> y ->
-    List.In (x, v) (list_replace y v' l) <-> List.In (x, v) l.
-  Proof.
-    induction l as [|(z, v'') l]; simpl.
-    - intuition congruence.
-    - intros Hs Hd.
-      case_eq (compare y z).
-      + intro He.
-        simpl.
-        rewrite compare_eq_iff in He.
-        destruct He.
-        intuition congruence.
-      + intro Hlt.
-        simpl.
-        intuition congruence.
-      + intro Hgt.
-        simpl.
-        rewrite IHl.
-        * intuition congruence.
-        * inversion Hs.
-          assumption.
-        * assumption.
-  Qed.
-
-  Lemma list_replace_in x v y v' l :
-    Sorted.StronglySorted (set.lt _ map_compare) l ->
-    List.In (x, v) (list_replace y v' l) <->
-      (match compare x y with Eq => v = v' | _ => List.In (x, v) l end).
-  Proof.
-    case_eq (compare x y).
-    - intro He.
-      apply compare_eq_iff in He.
-      destruct He.
-      apply list_replace_same.
-    - intros Hlt Hs.
-      apply list_replace_diff.
-      + assumption.
-      + intro He.
-        rewrite <- compare_eq_iff in He.
-        congruence.
-    - intros Hgt Hs.
-      apply list_replace_diff.
-      + assumption.
-      + intro He.
-        rewrite <- compare_eq_iff in He.
-        congruence.
-  Qed.
-
-  Definition list_update (x : A) (vo : option B) (l : list (A * B)) : list (A * B) :=
-    match vo with
-    | None => list_remove x l
-    | Some v => list_replace x v l
-    end.
-
-  Program Definition update (x : A) (vo : option B) (m : map) : map :=
-    let (l, _) := m in
-    exist _ (list_update x vo l) _.
-  Next Obligation.
-    destruct vo as [v|]; simpl.
-    - induction l as [|(k, v') l]; simpl.
-      + constructor.
-        * assumption.
-        * constructor.
-      + apply Sorted.StronglySorted_inv in H.
-        destruct H as (Hl, Hf).
-        specialize (IHl Hl).
-        case_eq (compare x k).
-        * intro He.
-          apply compare_eq_iff in He.
-          destruct He.
-          constructor.
-          {
-            assumption.
-          }
-          {
-            rewrite List.Forall_forall.
-            intros (z, v'') Hin.
-            rewrite List.Forall_forall in Hf.
-            specialize (Hf (z, v'') Hin).
-            generalize Hf.
-            unfold set.lt, map_compare.
-            auto.
-          }
-        * intro Hxk.
-          constructor.
-          {
-            constructor; assumption.
-          }
-          {
-            apply List.Forall_forall.
-            intros (z, v'') Hin.
-            rewrite List.Forall_forall in Hf.
-            specialize (Hf (z, v'')).
-            simpl in Hin.
-            destruct Hin as [He | Hin].
-            - injection He.
-              intros _ He2.
-              destruct He2.
-              exact Hxk.
-            - apply (lt_trans _ k).
-              + assumption.
-              + apply Hf.
-                assumption.
-          }
-        * intro Hgt.
-          constructor; try assumption.
-          apply List.Forall_forall.
-          intros (y,  v'').
-          rewrite list_replace_in; try assumption.
-          case_eq (compare y x).
-          {
-            intro He.
-            rewrite compare_eq_iff in He.
-            destruct He.
-            intros _.
-            unfold set.lt, map_compare.
-            apply set.compare_gt_lt; assumption.
-          }
-          {
-            intro Hlt.
-            rewrite List.Forall_forall in Hf.
-            exact (Hf (y, v'')).
-          }
-          {
-            intros Hgt2 _.
-            unfold set.lt, map_compare.
-            apply set.compare_gt_lt; try assumption.
-            apply (gt_trans _ x); assumption.
-          }
-    - induction l as [|(k, v') l]; simpl.
-      + assumption.
-      + case_eq (compare x k).
-        * intros _.
-          inversion H.
-          assumption.
-        * intros _.
-          assumption.
-        * apply Sorted.StronglySorted_inv in H.
-          destruct H as (Hs, Hf).
-          intro Hgt.
-          constructor.
-          {
-            auto.
-          }
-          {
-            apply List.Forall_forall.
-            intros (y, v'').
-            intro Hy.
-            apply remove_in in Hy.
-            rewrite List.Forall_forall in Hf.
-            exact (Hf _ Hy).
-          }
-  Qed.
-
-  Program Definition empty : map :=
-    exist _ nil _.
-  Next Obligation.
-    constructor.
-  Defined.
-
-  Fixpoint list_get (x : A) (l : list (A * B)) : option B :=
-    match l with
-    | nil => None
-    | cons y l =>
-      let (k, v) := y in
-      match compare x k with
-      | Lt => None
-      | Eq => Some v
-      | Gt => list_get x l
+  Fixpoint get_above (k : A) (v : B) (x : A) (m : sorted_map_above k) : option B :=
+    match compare x k with
+    | Lt => None
+    | Eq => Some v
+    | Gt =>
+      match m with
+      | sorted_map_sing _ => None
+      | sorted_map_cons _ k2 v2 _ m =>
+        get_above k2 v2 x m
       end
     end.
 
   Definition get (x : A) (m : map) : option B :=
-    let (l, _) := m in list_get x l.
+    match m with
+    | sorted_map_nil => None
+    | sorted_map_nonnil k v m =>
+      get_above k v x m
+    end.
 
-  Lemma StronglySorted_inv_iff (A' : Type) (R : A' -> A' -> Prop) (a : A')
-        (l : list A') :
-       Sorted.StronglySorted R (a :: l) <->
-       Sorted.StronglySorted R l /\ List.Forall (R a) l.
+  Lemma get_mem_false x m : mem x m = false <-> get x m = None.
   Proof.
-    split.
-    - apply Sorted.StronglySorted_inv.
-    - generalize Sorted.SSorted_cons.
-      intuition.
+    unfold mem, get.
+    destruct m.
+    - split; reflexivity.
+    - generalize dependent v.
+      induction s; intro v; simpl.
+      + destruct (compare x k); split; congruence.
+      + destruct (compare x k1); try (split; congruence).
+        apply IHs.
   Qed.
 
-  Lemma forall_cons (A' : Type) (P : A' -> Prop) (a : A') (l : list A') :
-    List.Forall P (cons a l) <-> (P a /\ List.Forall P l).
+  Lemma get_mem_absurd : false = true <-> (exists b : B, None = Some b).
   Proof.
-    split.
-    - intro H.
-      inversion H.
-      split; assumption.
-    - intros (HPa, Hf).
-      constructor; assumption.
+    split; intro H; [|destruct H]; discriminate.
   Qed.
 
-  Lemma list_sorted_map_fst (l : list (A * B)) :
-    Sorted.StronglySorted (fun x y => map_compare x y = Lt) l <->
-    Sorted.StronglySorted (fun x y => compare x y = Lt) (List.map fst l).
+  Lemma get_mem_base v : true = true <-> (exists b : B, Some v = Some b).
   Proof.
-    induction l as [|(x, v) l]; simpl.
-    - split; constructor.
-    - rewrite StronglySorted_inv_iff.
-      rewrite StronglySorted_inv_iff.
-      rewrite IHl.
-      clear IHl.
-      assert (List.Forall (fun y : A * B => map_compare (x, v) y = Lt) l <->
-              List.Forall (fun y : A => compare x y = Lt) (List.map fst l)) as H.
-      + induction l as [|(y, v') l]; simpl.
-        * split; constructor.
-        * rewrite forall_cons.
-          rewrite forall_cons.
-          rewrite IHl.
-          intuition.
-      + rewrite H.
-        intuition.
+    split; [| reflexivity].
+    intros _.
+    eexists; reflexivity.
   Qed.
 
-  Definition size (m : map) : nat :=
-    let (l, _) := m in List.length l.
-
-  Lemma list_get_lt a b l :
-    List.Forall (fun y => map_compare (a, b) y = Lt) l ->
-    Sorted.StronglySorted (fun x y => map_compare x y = Lt) l ->
-    list_get a l = None.
+  Lemma get_mem_true x m : mem x m = true <-> exists b, get x m = Some b.
   Proof.
-    intros Hf Hl.
-    destruct l as [|(a2, b2) l].
+    unfold mem, get.
+    destruct m.
+    - apply get_mem_absurd.
+    - generalize dependent v.
+      induction s; intro v; simpl.
+      + destruct (compare x k).
+        * apply get_mem_base.
+        * apply get_mem_absurd.
+        * apply get_mem_absurd.
+      + destruct (compare x k1).
+        * apply get_mem_base.
+        * apply get_mem_absurd.
+        * apply IHs.
+  Qed.
+
+  (* a return value of None means that the map is empty after removal *)
+  Fixpoint remove_above (k : A) (v : B) (x : A) (m : sorted_map_above k) :
+    option {k' & {v' : B & {m : sorted_map_above k' | compare k' k <> Lt}}} :=
+    match compare x k with
+    | Lt => Some (existT _ k (existT _ v (exist _ m (lt_irrefl k))))
+    | Eq =>
+      match m in (sorted_map_above k)
+            return (option {k' : A & {_ : B & {_ : sorted_map_above k' | compare k' k <> Lt}}}) with
+      | sorted_map_sing _ => None
+      | sorted_map_cons k1 k2 v2 H m =>
+        Some (existT _ k2 (existT _ v2 (exist _ m (lt_antisym k1 k2 H))))
+      end
+    | Gt =>
+      match m in (sorted_map_above k)
+            return (option {k' : A & {_ : B & {_ : sorted_map_above k' | compare k' k <> Lt}}}) with
+      | sorted_map_sing k => Some (existT _ k (existT _ v (exist _ (sorted_map_sing k) (lt_irrefl k))))
+      | sorted_map_cons k1 k2 v2 H m =>
+        match remove_above k2 v2 x m with
+        | Some (existT _ k3 (existT _ v3 (exist _ m' H'))) =>
+          let m'' := sorted_map_cons k1 k3 v3 (trans_lt_le _ _ _ H H') m' in
+          Some (existT _ k1 (existT _ v (exist _ m'' (lt_irrefl k1))))
+        | None =>
+          Some (existT _ k1 (existT _ v (exist _ (sorted_map_sing k1) (lt_irrefl k1))))
+        end
+      end
+    end.
+
+  Definition remove (x : A) (m : map) : map :=
+    match m with
+    | sorted_map_nil => sorted_map_nil
+    | sorted_map_nonnil k v m =>
+      match remove_above k v x m with
+      | None => sorted_map_nil
+      | Some (existT _ k' (existT _ v' (exist _ m' _))) =>
+        sorted_map_nonnil k' v' m'
+      end
+    end.
+
+  Lemma remove_above_absent k v x m :
+    get_above k v x m = None ->
+    exists H, remove_above k v x m = Some (existT _ k (existT _ v (exist _ m H))).
+  Proof.
+    generalize dependent v.
+    induction m; intro v; simpl.
+    - destruct (compare x k).
+      + discriminate.
+      + intros _.
+        eexists.
+        reflexivity.
+      + intros _.
+        eexists.
+        reflexivity.
+    - destruct (compare x k1).
+      + discriminate.
+      + intros _.
+        eexists.
+        reflexivity.
+      + intro Habsent.
+        specialize (IHm v2 Habsent).
+        destruct IHm as (Hlt, IHm).
+        eexists.
+        rewrite IHm.
+        repeat f_equal.
+        apply Eqdep_dec.UIP_dec.
+        decide equality.
+  Qed.
+
+  Lemma remove_absent x m : get x m = None -> remove x m = m.
+  Proof.
+    destruct m.
     - reflexivity.
-    - simpl.
-      rewrite List.Forall_forall in Hf.
-      specialize (Hf (a2, b2) (or_introl eq_refl)).
-      simpl in Hf.
-      rewrite Hf.
+    - intro Habsent.
+      specialize (remove_above_absent k v x s Habsent).
+      intros (H, He).
+      simpl.
+      rewrite He.
       reflexivity.
   Qed.
+
+  Lemma get_above_small x k v m : compare x k = Lt -> get_above k v x m = None.
+  Proof.
+    destruct m; simpl; intro H'; rewrite H'; reflexivity.
+  Qed.
+
+  Lemma get_above_eq x k v m : compare x k = Eq -> get_above k v x m = Some v.
+  Proof.
+    destruct m; simpl; intro H'; rewrite H'; reflexivity.
+  Qed.
+
+  Lemma remove_present_same x m :
+    get x (remove x m) = None.
+  Proof.
+    destruct m; simpl.
+    - reflexivity.
+    - generalize dependent v.
+      induction s; intro v; simpl.
+      + case_eq (compare x k); simpl.
+        * reflexivity.
+        * intro H; rewrite H; reflexivity.
+        * intro H; rewrite H; reflexivity.
+      + case_eq (compare x k1); simpl.
+        * intro He; apply compare_eq_iff in He; subst x.
+          apply get_above_small.
+          assumption.
+        * intro H'; rewrite H'; reflexivity.
+        * specialize (IHs v2).
+          destruct (remove_above k2 v2 x s) as [(k', (v', (m', H')))|]; simpl.
+          -- intro Hgt.
+             rewrite Hgt.
+             exact IHs.
+          -- intro Hgt; rewrite Hgt; reflexivity.
+  Qed.
+
+  Lemma unsome {X : Set} {x y : X} : Some x = Some y -> x = y.
+  Proof.
+    congruence.
+  Qed.
+
+  Ltac mytac :=
+    match goal with
+    | H : Some ?x = Some ?y |- _ => apply unsome in H
+    | H : existT _ ?x ?Hx = existT _ ?y ?Hy |- _ =>
+      apply error.existT_eq_3 in H; destruct H; subst; simpl
+    | H : exist _ ?x ?Hx = exist _ ?y ?Hy |- _ =>
+      apply error.exist_eq_3 in H; destruct H; subst; simpl
+    | H : eq_rec _ _ _ _ eq_refl = _ |- _ => simpl in H
+    end.
+
+  Lemma remove_above_none k v x m :
+    remove_above k v x m = None ->
+    m = sorted_map_sing k.
+  Proof.
+    destruct m; simpl.
+    - intro; reflexivity.
+    - destruct (compare x k1); try discriminate.
+      destruct (remove_above k2 v2 x m) as [(k3, (v3, (m3, H3)))|]; discriminate.
+  Qed.
+
+  Lemma remove_above_present_other k m : forall v x1 y1 x2 k' v' m' H,
+    get_above k v x1 m = Some y1 ->
+    remove_above k v x2 m = Some (existT _ k' (existT _ v' (exist _ m' H))) ->
+    get_above k' v' x1 m' = None ->
+    x1 = x2.
+  Proof.
+    induction m; intros v x1 y1 x2 k' v' m' H'; simpl.
+    - case_eq (compare x1 k); [|discriminate|discriminate].
+      intro He; apply compare_eq_iff in He; subst x1.
+      intros _.
+      case_eq (compare x2 k).
+      + discriminate.
+      + intros Hx2k He.
+        repeat mytac.
+        rewrite compare_refl.
+        discriminate.
+      + intros Hx2k He.
+        repeat mytac.
+        rewrite compare_refl.
+        discriminate.
+    - case_eq (compare x1 k1).
+      + intro He; apply compare_eq_iff in He; subst x1.
+        intros _.
+        case_eq (compare x2 k1).
+        * intros Hx2k1 _ _.
+          symmetry.
+          apply compare_eq_iff.
+          assumption.
+        * intros Hx2k1 He.
+          repeat mytac.
+          rewrite compare_refl.
+          discriminate.
+        * intros Hx2k1.
+          case_eq (remove_above k2 v2 x2 m).
+          -- intros (k'', (v'', (m'', H''))) Hm.
+             intro He.
+             repeat mytac.
+             rewrite compare_refl.
+             discriminate.
+          -- intros Hn He.
+             repeat mytac.
+             rewrite compare_refl.
+             discriminate.
+      + discriminate.
+      + case_eq (compare x2 k1).
+        * intro He; apply compare_eq_iff in He; subst x2.
+          intros.
+          repeat mytac.
+          congruence.
+        * intros.
+          repeat mytac.
+          simpl in H4.
+          rewrite H1 in H4.
+          congruence.
+        * intros Hx2 Hx1 Hmem.
+          case_eq (remove_above k2 v2 x2 m).
+          -- intros (k'', (v'', (m'', H''))) He Hm Hn.
+             specialize (IHm v2 x1 y1 x2 k'' v'' m'' H'' Hmem He).
+             repeat mytac.
+             simpl in Hn.
+             rewrite Hx1 in Hn.
+             apply IHm; assumption.
+          -- intros Hn _ _.
+             generalize (remove_above_none _ _ _ _ Hn).
+             intro; subst m.
+             simpl in Hn.
+             case_eq (compare x2 k2); intro Hx2k2; rewrite Hx2k2 in Hn;
+               try discriminate; clear Hn.
+             simpl in Hmem.
+             case_eq (compare x1 k2); intro Hx1k2; rewrite Hx1k2 in Hmem;
+               try discriminate; clear Hmem.
+             apply compare_eq_iff in Hx1k2.
+             apply compare_eq_iff in Hx2k2.
+             congruence.
+  Qed.
+
+  Lemma remove_above_present_untouched k m : forall v x1 y1 x2 k' v' m' H,
+      get_above k v x1 m = Some y1 ->
+      x1 <> x2 ->
+      remove_above k v x2 m = Some (existT _ k' (existT _ v' (exist _ m' H))) ->
+      get_above k' v' x1 m' = Some y1.
+  Proof.
+    induction m; intros v x1 y1 x2 k' v' m' H'; simpl.
+    - case_eq (compare x1 k); [|discriminate|discriminate].
+      intro He; apply compare_eq_iff in He; subst x1.
+      intro Hv.
+      case_eq (compare x2 k).
+      + discriminate.
+      + intros Hx2k Hneq He.
+        repeat mytac.
+        rewrite compare_refl.
+        reflexivity.
+      + intros Hx2k Hneq He.
+        repeat mytac.
+        rewrite compare_refl.
+        reflexivity.
+    - case_eq (compare x1 k1).
+      + intro He; apply compare_eq_iff in He; subst x1.
+        intro Hv.
+        case_eq (compare x2 k1).
+        * intros Hx2k1 Hk1x2 _.
+          apply compare_eq_iff in Hx2k1.
+          congruence.
+        * intros Hx2k1 Hneq He.
+          repeat mytac.
+          rewrite compare_refl.
+          reflexivity.
+        * intros Hx2k1 Hneq.
+          case_eq (remove_above k2 v2 x2 m).
+          -- intros (k'', (v'', (m'', H''))) Hm.
+             intro He.
+             repeat mytac.
+             rewrite compare_refl.
+             reflexivity.
+          -- intros Hn He.
+             repeat mytac.
+             rewrite compare_refl.
+             reflexivity.
+      + discriminate.
+      + case_eq (compare x2 k1).
+        * intro He; apply compare_eq_iff in He; subst x2.
+          intros.
+          repeat mytac.
+          assumption.
+        * intros.
+          repeat mytac.
+          rewrite H1.
+          assumption.
+        * intros Hx2 Hx1 Hmem.
+          case_eq (remove_above k2 v2 x2 m).
+          -- intros (k'', (v'', (m'', H''))) He Hm Hn.
+             specialize (IHm v2 x1 y1 x2 k'' v'' m'' H'' Hmem Hm He).
+             repeat mytac.
+             rewrite Hx1.
+             apply IHm; assumption.
+          -- intros Hn Hneq _.
+             generalize (remove_above_none _ _ _ _ Hn).
+             intro; subst m.
+             simpl in Hn.
+             case_eq (compare x2 k2); intro Hx2k2; rewrite Hx2k2 in Hn;
+               try discriminate; clear Hn.
+             simpl in Hmem.
+             case_eq (compare x1 k2); intro Hx1k2; rewrite Hx1k2 in Hmem;
+               try discriminate; clear Hmem.
+             apply compare_eq_iff in Hx1k2.
+             apply compare_eq_iff in Hx2k2.
+             congruence.
+  Qed.
+
+  Lemma remove_present_other x1 y1 x2 m :
+    get x1 m = Some y1 ->
+    get x1 (remove x2 m) = None ->
+    x1 = x2.
+  Proof.
+    destruct m; simpl.
+    - discriminate.
+    - case_eq (remove_above k v x2 s); simpl.
+      + intros (k', (v', (m', H'))) Hsome Hmemt Hmemf.
+        eapply remove_above_present_other; eassumption.
+      + intro Hnone.
+        generalize (remove_above_none _ _ _ _ Hnone).
+        intro; subst s.
+        simpl.
+        case_eq (compare x1 k); try discriminate.
+        simpl in Hnone.
+        case_eq (compare x2 k); intro Hx2; rewrite Hx2 in Hnone;
+          try discriminate; clear Hnone.
+        intro Hx1.
+        apply compare_eq_iff in Hx1.
+        apply compare_eq_iff in Hx2.
+        congruence.
+  Qed.
+
+  Lemma remove_present_untouched x1 y1 x2 m :
+    get x1 m = Some y1 ->
+    x1 <> x2 ->
+    get x1 (remove x2 m) = Some y1.
+  Proof.
+    destruct m; simpl.
+    - discriminate.
+    - case_eq (remove_above k v x2 s); simpl.
+      + intros (k', (v', (m', H'))) Hsome Hmemt Hmemf.
+        eapply remove_above_present_untouched; eassumption.
+      + intro Hnone.
+        generalize (remove_above_none _ _ _ _ Hnone).
+        intro; subst s.
+        simpl.
+        case_eq (compare x1 k); try discriminate.
+        simpl in Hnone.
+        case_eq (compare x2 k); intro Hx2; rewrite Hx2 in Hnone;
+          try discriminate; clear Hnone.
+        intro Hx1.
+        apply compare_eq_iff in Hx1.
+        apply compare_eq_iff in Hx2.
+        congruence.
+  Qed.
+
+
+  Definition min (k1 k2 : A) :=
+    match compare k1 k2 with
+    | Lt => k1
+    | Eq => k2
+    | Gt => k2
+    end.
+
+  Lemma min_not_lt_1 k1 k2 : compare k1 (min k1 k2) <> Lt.
+  Proof.
+    unfold min.
+    case_eq (compare k1 k2); intro H12.
+    - apply compare_eq_iff in H12.
+      subst k2.
+      apply lt_irrefl.
+    - apply lt_irrefl.
+    - congruence.
+  Qed.
+
+  Lemma min_not_lt_2 k1 k2 : compare k2 (min k1 k2) <> Lt.
+  Proof.
+    unfold min.
+    case_eq (compare k1 k2); intro H12.
+    - apply lt_irrefl.
+    - intro H21.
+      apply (lt_irrefl k1).
+      apply (lt_trans k1 k2 k1); assumption.
+    - apply lt_irrefl.
+  Qed.
+
+  Lemma min_lt k1 k2 k3 : compare k1 k2 = Lt -> compare k1 k3 = Lt -> compare k1 (min k2 k3) = Lt.
+  Proof.
+    unfold min.
+    destruct (compare k2 k3); intros; assumption.
+  Qed.
+
+  Fixpoint insert_above (k : A) (v : B) (x : A) (y : B) (m : sorted_map_above k) :
+    B * sorted_map_above (min x k) :=
+    match compare x k as c
+          return (compare x k = c ->
+                  B * sorted_map_above match c with
+                                       | Lt => x
+                                       | _ => k
+                                       end) with
+    | Eq => fun _  => (y, m)
+    | Lt => fun Hxk => (y, sorted_map_cons x k v Hxk m)
+    | Gt =>
+      fun Hxk =>
+        match m with
+        | sorted_map_sing k =>
+          fun Hxk =>
+            (v, sorted_map_cons k x y (gt_rev x k Hxk) (sorted_map_sing x))
+        | sorted_map_cons k1 k2 v2 H m =>
+          fun Hxk =>
+            let (v', m') := insert_above k2 v2 x y m in
+            (v, sorted_map_cons k1 (min x k2) v' (min_lt k1 x k2 (gt_rev x k1 Hxk) H) m')
+        end Hxk
+    end eq_refl.
+
+  Definition insert (x : A) (y : B) (m : map) : map :=
+    match m with
+    | sorted_map_nil => sorted_map_nonnil x y (sorted_map_sing x)
+    | sorted_map_nonnil k v m =>
+      let (v', m') := insert_above k v x y m in
+      sorted_map_nonnil (min x k) v' m'
+    end.
+
+  Definition insert_above_aux k v x y m c : compare x k = c -> B * sorted_map_above (match c with Lt => x | _ => k end) :=
+    match c return (compare x k = c -> B * sorted_map_above match c with Lt => x | _ => k end) with
+    | Eq => fun _ => (y, m)
+    | Lt => fun H => (y, sorted_map_cons x k v H m)
+    | Gt => match m with
+            | sorted_map_sing k =>
+              fun H => (v, sorted_map_cons k x y (gt_rev x k H) (sorted_map_sing x))
+            | sorted_map_cons k1 k2 v2 H' m =>
+              fun H =>
+                let (v', m') := insert_above k2 v2 x y m in
+                (v, sorted_map_cons k1 (min x k2) v' (min_lt k1 x k2 (gt_rev x k1 H) H') m')
+            end
+    end.
+
+  Lemma insert_above_aux_correct k v x y m :
+    insert_above k v x y m = insert_above_aux k v x y m (compare x k) eq_refl.
+  Proof.
+    destruct m; reflexivity.
+  Qed.
+
+  Lemma get_insert_above_aux x y v k m c He v' m' :
+    insert_above_aux k v x y m c He = (v', m') ->
+    get_above (match c with Lt => x | _ => k end) v' x m' = Some y.
+  Proof.
+    simpl in m.
+    generalize dependent v'.
+    induction m; intro v'; destruct c; simpl;
+      try (intro H'; injection H'; intros; subst; clear H'; simpl; rewrite He);
+      try rewrite compare_refl; try reflexivity.
+    case_eq (insert_above k2 v2 x y m); intros v'' m'' H''.
+    intro H'; injection H'; intros; subst; clear H'.
+    simpl.
+    rewrite He.
+    rewrite insert_above_aux_correct in H''.
+    generalize dependent m''.
+    unfold min.
+    case_eq (compare x k2); simpl.
+    - intros Hxk2 m'' Heq.
+      injection Heq; intros; subst; clear Heq.
+      apply get_above_eq.
+      assumption.
+    - intros Hxk2 m'' Heq.
+      injection Heq; intros; subst; clear Heq.
+      simpl.
+      rewrite compare_refl.
+      reflexivity.
+    - intros Hxk2 m''.
+      destruct m; simpl.
+      + intro Heq; injection Heq; intros; subst; clear Heq.
+        simpl.
+        rewrite Hxk2.
+        rewrite compare_refl.
+        reflexivity.
+      + case_eq (insert_above k2 v0 x y m).
+        intros v''' m''' Hi Heq.
+        injection Heq; intros; subst; clear Heq.
+        simpl.
+        rewrite Hxk2.
+        simpl in IHm.
+        rewrite Hi in IHm.
+        specialize (IHm Hxk2 _ v' eq_refl).
+        simpl in IHm.
+        rewrite Hxk2 in IHm.
+        exact IHm.
+  Qed.
+
+  Lemma get_insert x y m : get x (insert x y m) = Some y.
+  Proof.
+    destruct m; simpl.
+    - rewrite compare_refl.
+      reflexivity.
+    - case_eq (insert_above k v x y s); simpl.
+      intros v' m' H'.
+      rewrite insert_above_aux_correct in H'.
+      apply get_insert_above_aux in H'.
+      exact H'.
+  Qed.
+
+  Lemma get_insert_other_above_aux x y x' v k m c He v' m' :
+    x <> x' ->
+    insert_above_aux k v x y m c He = (v', m') ->
+    get_above (match c with Lt => x | _ => k end) v' x' m' =
+    get_above k v x' m.
+  Proof.
+    simpl in m.
+    intro Hneq.
+    assert (compare x' x = Lt \/ compare x' x = Gt) as Hneq2
+        by (apply compare_diff; congruence).
+    generalize dependent v'.
+    induction m; intro v'; destruct c; simpl;
+      try (intro H'; injection H'; intros; subst; clear H'; simpl).
+    - case_eq (compare x' k); try reflexivity.
+      intro Hx'.
+      apply compare_eq_iff in He.
+      apply compare_eq_iff in Hx'.
+      congruence.
+    - destruct Hneq2 as [Hneq2|Hneq2]; rewrite Hneq2; [|reflexivity].
+      rewrite (lt_trans _ _ _ Hneq2 He).
+      reflexivity.
+    - case_eq (compare x' k); try reflexivity.
+      destruct Hneq2 as [Hneq2|Hneq2]; rewrite Hneq2; reflexivity.
+    - case_eq (compare x' k1); try reflexivity.
+      apply compare_eq_iff in He.
+      intro Hx'.
+      apply compare_eq_iff in Hx'.
+      congruence.
+    - destruct Hneq2 as [Hneq2|Hneq2]; rewrite Hneq2; [|reflexivity].
+      rewrite (lt_trans _ _ _ Hneq2 He).
+      reflexivity.
+    - case_eq (insert_above k2 v2 x y m).
+      intros v'' m'' H''.
+      intro Heq; injection Heq; intros; subst; clear Heq.
+      simpl.
+      case_eq (compare x' k1); try reflexivity.
+      intro Hx'.
+      rewrite insert_above_aux_correct in H''.
+      generalize dependent m''.
+      unfold min.
+      case_eq (compare x k2); intros Hxk2 m'' Hi.
+      + simpl in Hi.
+        injection Hi; intros; subst; clear Hi.
+        apply compare_eq_iff in Hxk2; subst x.
+        destruct Hneq2 as [Hneq2|Hneq2].
+        * rewrite get_above_small; [|assumption].
+          rewrite get_above_small; [|assumption].
+          reflexivity.
+        * destruct m''; simpl; rewrite Hneq2; reflexivity.
+      + simpl in Hi.
+        injection Hi; intros; subst; clear Hi.
+        simpl.
+        destruct Hneq2 as [Hneq2|Hneq2]; rewrite Hneq2.
+        * rewrite get_above_small; [reflexivity|].
+          apply (lt_trans _ x _); assumption.
+        * reflexivity.
+      + simpl in Hi.
+        destruct m.
+        * injection Hi; intros; subst; clear Hi.
+          simpl.
+          destruct (compare x' k); try reflexivity.
+          destruct Hneq2 as [Hneq2|Hneq2]; rewrite Hneq2; reflexivity.
+        * case_eq (insert_above k2 v0 x y m).
+          intros v''' m''' H'''.
+          simpl.
+          rewrite H''' in Hi.
+          injection Hi; intros; subst; clear Hi.
+          simpl.
+          case_eq (compare x' k0); try reflexivity.
+          simpl in IHm.
+          intro Hx'k0.
+          rewrite Hx'k0 in IHm.
+          rewrite H''' in IHm.
+          specialize (IHm Hxk2 _ _ eq_refl).
+          simpl in IHm.
+          rewrite Hx'k0 in IHm.
+          assumption.
+  Qed.
+
+  Lemma get_insert_other x y x' m : x <> x' -> get x' (insert x y m) = get x' m.
+  Proof.
+    intro Hneq.
+    assert (compare x' x = Lt \/ compare x' x = Gt) as Hneq2
+        by (apply compare_diff; congruence).
+    destruct m; simpl.
+    - destruct Hneq2 as [Hneq2|Hneq2]; rewrite Hneq2; reflexivity.
+    - case_eq (insert_above k v x y s); simpl.
+      intros v' m' H'.
+      rewrite insert_above_aux_correct in H'.
+      eapply get_insert_other_above_aux in H'; eassumption.
+  Qed.
+
+  Definition update (x : A) (vo : option B) (m : map) : map :=
+    match vo with
+    | None => remove x m
+    | Some y => insert x y m
+    end.
+
+  Definition empty : map := sorted_map_nil.
+
+  Fixpoint size_above k (m : sorted_map_above k) : nat :=
+    match m with
+    | sorted_map_sing _ => 1
+    | sorted_map_cons _ _ _ _ m =>
+      S (size_above _ m)
+    end.
+
+  Definition size (m : map) : nat :=
+    match m with
+    | sorted_map_nil => 0
+    | sorted_map_nonnil _ _ m => S (size_above _ m)
+    end.
 
   Lemma extensionality (m1 m2 : map) :
     (forall x, get x m1 = get x m2) -> m1 = m2.
   Proof.
-    destruct m1 as (l1, H1).
-    destruct m2 as (l2, H2).
-    simpl.
-    intro Hf.
-    assert (l1 = l2).
-    - generalize l2 H2 Hf; clear l2 H2 Hf; induction l1 as [|(a1, b1) l1]; intros [|(a2, b2) l2] H2 Hf.
-      + reflexivity.
-      + exfalso.
-        specialize (Hf a2).
-        simpl in Hf.
-        rewrite compare_refl in Hf.
-        discriminate.
-      + exfalso.
-        specialize (Hf a1).
-        simpl in Hf.
-        rewrite compare_refl in Hf.
-        discriminate.
-      + assert (a1 = a2 /\ b1 = b2).
-        * generalize (Hf a1); intro Ha1.
-          simpl in Ha1.
-          rewrite compare_refl in Ha1.
-          generalize (Hf a2); intro Ha2.
-          simpl in Ha2.
-          rewrite compare_refl in Ha2.
-          case_eq (compare a1 a2).
-          -- intro He.
-             rewrite compare_eq_iff in He.
-             split; [assumption|].
-             subst a2.
-             rewrite compare_refl in Ha1.
-             injection Ha1.
-             auto.
-          -- intro Hlt.
-             rewrite Hlt in Ha1.
+    destruct m1 as [|k1 v1 m1]; destruct m2 as [|k2 v2 m2].
+    - reflexivity.
+    - intro H; exfalso.
+      specialize (H k2).
+      simpl in H.
+      rewrite get_above_eq in H.
+      + discriminate.
+      + apply compare_refl.
+    - intro H; exfalso.
+      specialize (H k1).
+      simpl in H.
+      rewrite get_above_eq in H.
+      + discriminate.
+      + apply compare_refl.
+    - intro H.
+      simpl in H.
+      case_eq (compare k1 k2).
+      + intro Hk1k2.
+        apply compare_eq_iff in Hk1k2.
+        subst k2.
+        generalize (H k1); intro H2.
+        rewrite get_above_eq in H2; [|apply compare_refl].
+        rewrite get_above_eq in H2; [|apply compare_refl].
+        apply unsome in H2.
+        subst v2.
+        f_equal.
+        generalize dependent m2.
+        generalize dependent v1.
+        induction m1 as [k1|k1 k1' v1' H1]; simpl; intros v1 m2 H.
+        * destruct m2 as [k|k1 k2 v2 H2]; [reflexivity|].
+          specialize (H k2).
+          simpl in H.
+          rewrite (lt_rev _ _ H2) in H.
+          rewrite get_above_eq in H; [|apply compare_refl].
+          discriminate.
+        * destruct m2 as [k|k1 k2 v2 H2].
+          -- simpl in H.
+             specialize (H k1').
+             rewrite (lt_rev _ _ H1) in H.
+             rewrite get_above_eq in H; [|apply compare_refl].
              discriminate.
-          -- intro Hgt.
-             rewrite Hgt in Ha1.
-             rewrite <- set.compare_gt_lt in Hgt;
-               [|assumption|assumption|assumption].
-             rewrite Hgt in Ha2.
-             discriminate.
-        * destruct H; subst a2; subst b2.
-          f_equal.
-          apply IHl1.
-          -- inversion H1.
-             assumption.
-          -- inversion H2.
-             assumption.
-          -- intro a3.
-             specialize (Hf a3).
-             simpl in Hf.
-             case_eq (compare a3 a1).
-             ** intro Heq.
-                rewrite compare_eq_iff in Heq.
-                subst a3.
-                rewrite (list_get_lt a1 b1 l1); [|inversion H1; assumption|inversion H1; assumption].
-                rewrite (list_get_lt a1 b1 l2); [|inversion H2; assumption|inversion H2; assumption].
-                reflexivity.
-             ** intro Hlt.
-                rewrite (list_get_lt a3 b1 l1);
-                  [rewrite (list_get_lt a3 b1 l2)| |].
-                --- reflexivity.
-                --- apply (@List.Forall_impl _ (fun y => map_compare (a1, b1) y = Lt)); [|inversion H2; assumption].
-                    intros (a4, b4).
-                    simpl.
-                    apply lt_trans.
-                    assumption.
-                --- inversion H2; assumption.
-                --- apply (@List.Forall_impl _ (fun y => map_compare (a1, b1) y = Lt)); [|inversion H1; assumption].
-                    intros (a4, b4).
-                    simpl.
-                    apply lt_trans.
-                    assumption.
-                --- inversion H1; assumption.
-             ** intro Hgt.
-                rewrite Hgt in Hf.
-                exact Hf.
-    - destruct H.
-      f_equal.
-      apply set.sorted_irrel.
+          -- simpl in H.
+             generalize (H k1'); intro H3.
+             rewrite (lt_rev _ _ H1) in H3.
+             rewrite get_above_eq in H3; [|apply compare_refl].
+             generalize (H k2); intro H4.
+             rewrite (lt_rev _ _ H2) in H4.
+             rewrite (get_above_eq k2 k2) in H4; [|apply compare_refl].
+             case_eq (compare k1' k2).
+             ++ intro Hk1k2.
+                apply compare_eq_iff in Hk1k2.
+                subst k2.
+                rewrite get_above_eq in H4; [|apply compare_refl].
+                apply unsome in H4.
+                subst v2.
+                f_equal.
+                ** apply Eqdep_dec.UIP_dec.
+                   decide equality.
+                ** apply (IHm1 v1').
+                   intro x.
+                   case_eq (compare x k1); intro Hx.
+                   --- apply compare_eq_iff in Hx.
+                       subst x.
+                       rewrite get_above_small; [|assumption].
+                       rewrite get_above_small; [|assumption].
+                       reflexivity.
+                   --- assert (compare x k1' = Lt) as Hx' by (eapply lt_trans; eassumption).
+                       rewrite get_above_small; [|assumption].
+                       rewrite get_above_small; [|assumption].
+                       reflexivity.
+                   --- specialize (H x).
+                       rewrite Hx in H.
+                       exact H.
+             ++ intro H5; rewrite get_above_small in H3; [discriminate|assumption].
+             ++ intro H5; apply gt_rev in H5; rewrite get_above_small in H4; [discriminate|assumption].
+      + intro Hk1k2.
+        specialize (H k1).
+        rewrite get_above_eq in H; [|apply compare_refl].
+        rewrite get_above_small in H; [|assumption].
+        discriminate.
+      + intro Hk1k2.
+        apply gt_rev in Hk1k2.
+        specialize (H k2).
+        rewrite get_above_small in H; [|assumption].
+        rewrite get_above_eq in H; [|apply compare_refl].
+        discriminate.
   Qed.
 
   (* Interesting lemmas to use when working with maps *)
 
-  Lemma map_getmem : forall k m v, 
+  Lemma map_getmem k m v :
       get k m = Some v -> mem k m.
   Proof.
-    intros.
-    destruct m as [l]. simpl. simpl in H.
-    induction l.
-    - (* nil *)
-      simpl in H. inversion H.
-    - (* h :: t *)
-      simpl. simpl in H.
-      destruct a as [k' v']. destruct (compare k k').
-      + (* Eq *) constructor.
-      + (* Lt *) inversion H.
-      + (* Gt *) apply IHl. inversion s. assumption. assumption.
+    intro H.
+    apply Bool.Is_true_eq_left.
+    rewrite get_mem_true.
+    exists v.
+    assumption.
   Qed.
 
-  Lemma map_memget : forall k m,
+  Lemma map_memget k m :
       mem k m -> exists v, get k m = Some v.
   Proof.
-    intros.
-    destruct m as [l]. simpl. simpl in H.
-    induction l.
-    - (* nil *)
-      exfalso. simpl in H. inversion H.
-    - (* h :: t *)
-      inversion s; subst.
-      specialize (IHl H2).
-      simpl in H. simpl.
-      destruct a as [k' v']. destruct (compare k k').
-      + (* Eq *) exists v'. reflexivity.
-      + (* Lt *) inversion H.
-      + (* Gt *)
-        specialize (IHl H). destruct IHl as [v'' IHl].
-        exists v''. assumption.
+    intro H.
+    apply get_mem_true.
+    apply Bool.Is_true_eq_true.
+    exact H.
   Qed.
 
-  Lemma map_updateeq : forall k m v,
+  Lemma map_updateeq k m v :
       get k (update k (Some v) m) = (Some v).
   Proof.
-    intros.
-    destruct m as [l]. unfold get, update.
-    assert ((compare k k) = Eq) as Hkk by (apply compare_eq_iff; reflexivity).
-    induction l.
-    - (* nil *)
-      simpl. rewrite Hkk. reflexivity.
-    - (* h :: t *)
-      simpl. inversion s; subst.
-      specialize (IHl H1). simpl in IHl.
-      destruct a as [k' v'].
-      destruct (compare k k') eqn:Hkk'; simpl.
-      + (* Eq *) simpl. rewrite Hkk. reflexivity.
-      + (* Lt *) simpl. rewrite Hkk. reflexivity.
-      + (* Gt *) rewrite Hkk'. assumption.
+    apply get_insert.
   Qed.
 
-  Lemma map_updateneq : forall k k' m v,
+  Lemma map_updateneq k k' m v :
       k <> k' ->
       get k' (update k (Some v) m) =
       get k' m.
   Proof.
-    intros.
-    destruct m as [l]. unfold get, update; simpl.
-    induction l; simpl.
-    - (* nil *)
-      destruct (compare k' k) eqn:Hcp; try reflexivity.
-      apply compare_eq_iff in Hcp. symmetry in Hcp. contradiction.
-    - (* h :: t *)
-      inversion s; subst.
-      specialize (IHl H2). simpl in IHl.
-      destruct a as [k'' v''].
-      destruct (compare k k'') eqn:Hkk''; destruct (compare k' k'') eqn:Hk'k''; simpl;
-        try apply compare_eq_iff in Hkk''; try apply compare_eq_iff in Hk'k''; subst;
-          assert (compare k'' k'' = Eq) as Hk'' by (apply compare_eq_iff; reflexivity);
-          try (rewrite Hk'k''; auto).
-      + contradiction.
-      + rewrite Hk''. apply set.compare_gt_lt in Hkk''; try assumption.
-        rewrite Hkk''. reflexivity.
-      + destruct (compare k' k) eqn:Hk'k; try reflexivity.
-        apply compare_eq_iff in Hk'k. symmetry in Hk'k. contradiction.
-      + apply set.compare_gt_lt in Hkk''; try assumption.
-        unfold Relations_1.Transitive in gt_trans.
-        assert (compare k' k = Gt) as Hk'k by (eapply gt_trans; eassumption).
-        rewrite Hk'k. reflexivity.
-      + rewrite Hk''. reflexivity.
+    apply get_insert_other.
   Qed.
 
-  Lemma map_updateSome_spec : forall k v m nm,
+  Lemma map_updateSome_spec k v m nm :
       nm = update k (Some v) m <->
       (get k nm = (Some v) /\
        (forall k', k <> k' -> map.get k' nm = map.get k' m)).
   Proof.
-    intros. split.
+    simpl.
+    split.
     - (* -> *)
       intros Hnm. subst. split.
       apply map_updateeq. intros k' Hdiff. apply map_updateneq. assumption.
@@ -626,127 +986,291 @@ Section map.
         apply map_updateneq. assumption.
   Qed.
 
-  Lemma map_updatemem : forall k m v,
+  Lemma map_updatemem k m v :
       mem k m ->
       forall k', mem k (map.update k' (Some v) m).
   Proof.
-    intros.
-    destruct m as [l]. unfold get, update. simpl. simpl in H.
-    induction l; simpl; simpl in H.
-    - (* nil *) inversion H.
-    - (* h :: t *)
-      inversion s; subst. specialize (IHl H2).
-      destruct a as [k'' v''].
-      destruct (compare k k'') eqn:Hkk''; destruct (compare k' k'') eqn:Hk'k'';
-        simpl in H; simpl;
-          try rewrite compare_eq_iff in Hkk''; try rewrite compare_eq_iff in Hk'k''; subst;
-            assert (compare k'' k'' = Eq) as Hk'' by (apply compare_eq_iff; reflexivity);
-            try inversion H;
-            try rewrite Hk''; try rewrite Hkk''; try exact ITT.
-      + constructor.
-      + apply set.compare_gt_lt in Hk'k''; try assumption.
-        rewrite Hk'k''.
-        constructor.
-      + constructor.
-      + assumption.
-      + apply set.compare_gt_lt in Hk'k''; try assumption.
-        rewrite (gt_trans _ _ _ Hkk'' Hk'k'').
-        assumption.
-      + apply IHl; assumption.
+    intros Hmem k'.
+    simpl.
+    destruct (eq_dec k k').
+    - subst k'.
+      apply (map_getmem _ _ v).
+      apply get_insert.
+    - apply map_memget in Hmem.
+      destruct Hmem as (v', Hget).
+      apply (map_getmem _ _ v').
+      rewrite <- Hget.
+      apply get_insert_other.
+      congruence.
   Qed.
 
-  Ltac comparison_case k1 k2 H Hmem :=
-    case_eq (compare k1 k2); intro H; simpl in Hmem; try rewrite H in Hmem;
-    [ rewrite compare_eq_iff in H; try assumption | | ].
-
-  Lemma map_updatemem_rev : forall k k' m v,
+  Lemma map_updatemem_rev k k' m v :
       k <> k' ->
       mem k (map.update k' (Some v) m) ->
       mem k m.
   Proof.
-    intros k k' m v Hkk' Hmem.
-    destruct m as [l].
-    simpl in *.
-    induction l as [|(k'', v'') l]; simpl in *.
-    - (* nil *)
-      comparison_case k k' H Hmem.
-      + congruence.
-      + inversion Hmem.
-      + inversion Hmem.
-    - (* h :: t *)
-      comparison_case k' k'' Hk'k'' Hmem;
-        [ subst k'' | comparison_case k k'' Hkk'' Hmem | comparison_case k k'' Hkk'' Hmem ]; simpl in Hmem; comparison_case k k' Hckk' Hmem;
-          try constructor; simpl in *; try (exact Hmem); try (destruct Hmem);
-            try congruence;
-            inversion s; apply IHl; assumption.
+    intros Hkk' Hmem.
+    apply map_memget in Hmem.
+    destruct Hmem as (v', Hget).
+    apply (map_getmem _ _ v').
+    rewrite <- Hget.
+    symmetry.
+    apply get_insert_other.
+    congruence.
+  Qed.
+
+  Definition destruct (m : map) : option (A * B * map) :=
+    match m with
+    | sorted_map_nil => None
+    | sorted_map_nonnil k v m =>
+      Some (k, v,
+            match m with
+            | sorted_map_sing k => sorted_map_nil
+            | sorted_map_cons k1 k2 v2 _ m =>
+              sorted_map_nonnil k2 v2 m
+            end)
+    end.
+
+  (* Conversions from and to lists *)
+  Fixpoint to_list_above {k} (m : sorted_map_above k) : list (A * B) :=
+    match m with
+    | sorted_map_sing x => nil
+    | sorted_map_cons k1 k2 v2 H m => cons (k2, v2) (to_list_above m)
+    end.
+
+  Definition to_list (m : map) : list (A * B) :=
+    match m with
+    | sorted_map_nil => nil
+    | sorted_map_nonnil k v m => cons (k, v) (to_list_above m)
+    end.
+
+  Definition map_lt : (A * B) -> (A * B) -> Prop :=
+    fun '(k1, _) '(k2, _) => compare k1 k2 = Lt.
+
+  Lemma to_list_above_is_locally_sorted k v (m : sorted_map_above k) :
+    Sorted.LocallySorted map_lt (cons (k, v) (to_list_above m)).
+  Proof.
+    generalize dependent v.
+    induction m.
+    - constructor.
+    - simpl.
+      constructor.
+      + apply IHm.
+      + assumption.
+  Defined.
+
+  Lemma to_list_is_locally_sorted (m : map) :
+    Sorted.LocallySorted map_lt (to_list m).
+  Proof.
+    destruct m.
+    - constructor.
+    - apply to_list_above_is_locally_sorted.
+  Defined.
+
+  Definition locally_sorted_proj1 {X lt x y} {l : list X} :
+    Sorted.LocallySorted lt (cons x (cons y l)) ->
+    Sorted.LocallySorted lt (cons y l).
+  Proof.
+    intro H; inversion H; assumption.
+  Defined.
+
+  Definition locally_sorted_proj2 {X lt x y} {l : list X} :
+    Sorted.LocallySorted lt (cons x (cons y l)) ->
+    lt x y.
+  Proof.
+    intro H; inversion H; assumption.
+  Defined.
+
+  Fixpoint of_list_above k v (l : list (A * B)) {struct l} :
+    Sorted.LocallySorted map_lt (cons (k, v) l) -> sorted_map_above k :=
+    match l with
+    | nil => fun _ => sorted_map_sing k
+    | cons (k2, v2) l =>
+      fun H =>
+        sorted_map_cons
+          k k2 v2
+          (locally_sorted_proj2 H)
+          (of_list_above k2 v2 l (locally_sorted_proj1 H))
+    end.
+
+  Definition of_list (l : list (A * B)) :
+    Sorted.LocallySorted map_lt l -> map :=
+    match l with
+    | nil => fun _ => sorted_map_nil
+    | cons (k, v) l =>
+      fun H =>
+        sorted_map_nonnil k v (of_list_above k v l H)
+    end.
+
+  Lemma of_to_list_above k v (l : list (A * B)) H :
+    to_list_above (of_list_above k v l H) = l.
+  Proof.
+    generalize dependent v.
+    generalize dependent k.
+    induction l as [|(k2, v2) l].
+    - reflexivity.
+    - simpl.
+      intros k1 v1 H.
+      f_equal.
+      apply IHl.
+  Qed.
+
+  Lemma of_to_list (l : list (A * B)) H :
+    to_list (of_list l H) = l.
+  Proof.
+    destruct l as [|(k, v) l].
+    - reflexivity.
+    - simpl.
+      f_equal.
+      apply of_to_list_above.
+  Qed.
+
+  Lemma to_of_list_above k v (m : sorted_map_above k) :
+    of_list_above k v (to_list_above m) (to_list_above_is_locally_sorted k v m) = m.
+  Proof.
+    generalize dependent v.
+    induction m.
+    - reflexivity.
+    - intro v1.
+      simpl.
+      f_equal.
+      apply IHm.
+  Qed.
+
+  Lemma to_of_list (m : sorted_map) :
+    of_list (to_list m) (to_list_is_locally_sorted m) = m.
+  Proof.
+    destruct m.
+    - reflexivity.
+    - simpl.
+      f_equal.
+      apply to_of_list_above.
+  Qed.
+
+  Lemma sorted_dec l : {Sorted.LocallySorted map_lt l} + {~ Sorted.LocallySorted map_lt l}.
+  Proof.
+    induction l as [|(k1, v1) l].
+    - left.
+      constructor.
+    - destruct l as [|(k2, v2) l].
+      + left.
+        constructor.
+      + case_eq (compare k1 k2).
+        * intro Hk.
+          right.
+          intro H.
+          apply locally_sorted_proj2 in H.
+          simpl in H.
+          congruence.
+        * intro Hk.
+          destruct IHl.
+          -- left.
+             constructor; assumption.
+          -- right.
+             intro H.
+             apply locally_sorted_proj1 in H.
+             contradiction.
+        * intro Hk.
+          right.
+          intro H.
+          apply locally_sorted_proj2 in H.
+          simpl in H.
+          congruence.
+  Defined.
+
+  Lemma sorted_inversion l (H : Sorted.LocallySorted map_lt l) :
+    match l, H with
+    | nil, H => H = Sorted.LSorted_nil _
+    | cons (k, v) nil, H => H = Sorted.LSorted_cons1 _ _
+    | cons (k1, v1) (cons (k2, v2) l), H =>
+      H = Sorted.LSorted_consn _
+            (locally_sorted_proj1 H) (locally_sorted_proj2 H)
+    end.
+  Proof.
+    destruct H.
+    - reflexivity.
+    - destruct a as (k, v).
+      reflexivity.
+    - destruct a as (k1, v1).
+      destruct b as (k2, v2).
+      reflexivity.
+  Qed.
+
+  Lemma lt_irrel k1 k2 : forall H1 H2 : compare k1 k2 = Lt, H1 = H2.
+  Proof.
+    apply Eqdep_dec.UIP_dec.
+    decide equality.
+  Qed.
+
+  Lemma sorted_irrel l (H1 H2 : Sorted.LocallySorted map_lt l) : H1 = H2.
+  Proof.
+    induction l as [|(k1, v1) l].
+    - rewrite (sorted_inversion _ H1).
+      rewrite (sorted_inversion _ H2).
+      reflexivity.
+    - destruct l as [|(k2, v2) l].
+      + rewrite (sorted_inversion _ H1).
+        rewrite (sorted_inversion _ H2).
+        reflexivity.
+      + rewrite (sorted_inversion _ H1).
+        rewrite (sorted_inversion _ H2).
+        f_equal.
+        * apply IHl.
+        * apply lt_irrel.
+  Qed.
+
+  Lemma sorted_tail k v l :
+    Sorted.LocallySorted map_lt (cons (k, v) l) ->
+    Sorted.LocallySorted map_lt l.
+  Proof.
+    destruct l as [|(k2, v2) l].
+    - intros _.
+      constructor.
+    - apply locally_sorted_proj1.
   Qed.
 
 End map.
 
-Fixpoint list_map (B B' : Set) (f : B -> M B') (l : list B) : M (list B') :=
-  match l with
-  | nil => Return nil
-  | cons x l =>
-    let! b' := f x in
-    let! l' := list_map _ _ f l in
-    Return (cons b' l')
+Fixpoint map_fun_above (A B B' : Set) compare (f : B -> M B') k (m : sorted_map_above A B compare k)
+  : M (sorted_map_above A B' compare k) :=
+  match m with
+  | sorted_map_sing _ _ _ k =>
+    Return (sorted_map_sing _ _ _ k)
+  | sorted_map_cons _ _ _ k1 k2 v2 H m =>
+    let! v2' := f v2 in
+    let! m' := map_fun_above A B B' compare f k2 m in
+    Return (sorted_map_cons _ _ _ k1 k2 v2' H m')
   end.
 
-Definition list_map_pair (A B B' : Set) (f : (A * B) -> M B') :
-  list (A * B) -> M (list (A * B')) :=
-  list_map (A * B) (A * B')
-           (fun ab => let! b' := f ab in Return (fst ab, b')).
-
-Lemma list_map_fst A B B' f l l' :
-  list_map_pair A B B' f l = Return l' ->
-  List.map fst l = List.map fst l'.
-Proof.
-  generalize l'. clear l'.
-  induction l as [|(x, v) l].
-  - simpl.
-    intros l' H.
-    injection H.
-    intro He.
-    destruct He.
-    reflexivity.
-  - simpl.
-    intro l'.
-    unfold list_map_pair.
-    simpl.
-    case_eq (f (x, v)); simpl; try congruence.
-    intros b' He.
-    case_eq (list_map (A * B) (A * B') (fun ab : A * B =>
-        let! b'0 : B' := f ab in Return (fst ab, b'0)) l); simpl; try congruence.
-    intros l'' He2.
-    specialize (IHl l'').
-    intro H3.
-    injection H3.
-    intro Hl'.
-    destruct Hl'.
-    simpl.
-    f_equal.
-    apply IHl.
-    assumption.
-Qed.
-
-Program Definition map_fun_aux (A B B' : Set) compare (f : A * B -> M B') (l : list (A * B))
-        (H : Sorted.StronglySorted (fun x y => map_compare _ _ compare x y = Lt) l): M (map A B' compare) :=
-  match (list_map_pair _ _ _ f l) with
-  | Return l' => Return (exist _ l' _)
-  | Failed _ e => Failed _ e
+Definition map_fun (A B B' : Set) compare (f : B -> M B') (m : map A B compare)
+  : M (map A B' compare) :=
+  match m with
+  | sorted_map_nil _ _ _ =>
+    Return (sorted_map_nil _ _ _)
+  | sorted_map_nonnil _ _ _ k v m =>
+    let! v' := f v in
+    let! m' := map_fun_above A B B' compare f k m in
+    Return (sorted_map_nonnil _ _ _ k v' m')
   end.
-Next Obligation.
-  unfold set.lt.
-  rewrite list_sorted_map_fst.
-  rewrite <- (list_map_fst _ _ _ f l).
-  + apply list_sorted_map_fst.
-    assumption.
-  + symmetry.
-    assumption.
-Defined.
 
-Definition map_fun (A B B' : Set) comp
-  (f : A * B -> M B')
-  (m : map A B comp) : M (map A B' comp) :=
-  let (l, H) := m in
-  map_fun_aux _ _ _ comp f l H.
+Fixpoint map_fun_above_pure (A B B' : Set) compare (f : B -> B') k (m : sorted_map_above A B compare k)
+  : sorted_map_above A B' compare k :=
+  match m with
+  | sorted_map_sing _ _ _ k =>
+    sorted_map_sing _ _ _ k
+  | sorted_map_cons _ _ _ k1 k2 v2 H m =>
+    let v2' := f v2 in
+    let m' := map_fun_above_pure A B B' compare f k2 m in
+    sorted_map_cons _ _ _ k1 k2 v2' H m'
+  end.
+
+Definition map_fun_pure (A B B' : Set) compare (f : B -> B') (m : map A B compare)
+  : map A B' compare :=
+  match m with
+  | sorted_map_nil _ _ _ =>
+    sorted_map_nil _ _ _
+  | sorted_map_nonnil _ _ _ k v m =>
+    let v' := f v in
+    let m' := map_fun_above_pure A B B' compare f k m in
+    sorted_map_nonnil _ _ _ k v' m'
+  end.
